

Q7. $S := \mathbb{R} \setminus \{-1\}$

Define binary operation $*$ on S by
 $a, b \in S \quad a * b := a + b + ab.$

Prove $(S, *)$ is an abelian group

We showed $*$ is closed on S

i.e. $a, b \in S \Rightarrow a * b \in S$

\swarrow $b + c + bc$

Associativity

claim $(a * b) * c = a * (b * c)$

Proof:

$(a * b) * c = (a + b + ab) * c$, def of $*$

$= (a + b + ab) + c + (a + b + ab)c$
 , by def of $*$

$= a + b + ab + c + ac + bc + abc$

$= a + \underbrace{ab} + (b + c + bc) + \underbrace{ac} + \underbrace{abc}$

$= a + (b + c + bc) + a(b + c + bc)$

$= a * (b + c + bc)$, def of $*$

$$= a * (b * c)$$

Pause: Claim $x * y = y * x$.

$$\boxed{x * y} = x + y + xy, \text{ def of } *$$

$$= y + x + yx, \text{ since } +, \cdot \text{ commutative on } \mathbb{R}.$$

$$= \boxed{y * x}$$

$(S, *)$ will be abelian.

Identity The identity for $*$ is 0.
For any $a \in S$.

$$\text{since } a * 0 = a + 0 + a \cdot 0 = a$$

Inverses For $a \in S$, is there an $a^{-1} \in S$?

Claim: $a^{-1} = \frac{-a}{1+a}$. Good.

Let's discover this.

We want

$$a * a^{-1} = 0$$

$$\Leftrightarrow a + a^{-1} + aa^{-1} = 0$$

$$\Leftrightarrow a + a^{-1}(1+a) = 0$$

$$\Leftrightarrow a^{-1} = \frac{-a}{1+a}, \text{ and } 1+a \neq 0$$

So yes there is an inverse. in S
 (note also $\frac{-a}{1+a} \neq -1$)

Therefore $(S, *)$ is a group.

and abelian property proved above. ~~###~~

Basic properties that come straight from the definition

Prop 3.17 The identity element is unique.

Proof Suppose there are two

identities e_1, e_2 . Consider the

product $e_1 e_2$ element

$$e_1 = e_1 e_2 = e_2$$

(Writing the group product without \circ)

e_2 is an identity

↓ some e_1 is an identity

So $e_1 = e_2$.

Prop 3.18 Inverses are unique.

Proof Let $g \in G$, Suppose g', g'' are both inverses of g .

$$\text{Consider } g'' = g' g g'' = g'$$

Prop 3.19 $\forall a, b \in G$

$$(ab)^{-1} = b^{-1} a^{-1}$$

- Seen in linear algebra for mat. mult.
- Seen in reality.

Prop 3.20 $\forall a \in G \quad (a^{-1})^{-1} = a$

Prop 3.21, 3.22.

$$3.21 \quad ax = b \Rightarrow x = a^{-1}b$$

$$a(a^{-1}b) = aa^{-1}b = eb = b$$

$$xa=b \Rightarrow x=ba^{-1}$$

$$ba=ca \Rightarrow b=c$$

Proof

$$ba=ca$$

$$\Leftrightarrow b = caa^{-1}, \text{ using Prop 3.21.}$$

$$= ce$$

$$= c$$

Warning.

$$\nexists \quad ba=ac$$

does not imply that $b=c$.

We can say

$$ba=ac \Rightarrow baa^{-1} = aca^{-1}$$

$$\Rightarrow b = aca^{-1}$$

is always be aware of abelian
status of your group

We can use exponential notation

For $g \in (G, 0)$

g^n will mean, for $n > 0$

$$g^n := \underbrace{g \circ g \circ g \circ \dots \circ g}_{n \text{ gs here.}}$$

and can extend to this with the definitions

$$g^0 := e.$$

and for $n > 0$

$$g^{-n} := \underbrace{g^{-1} \circ g^{-1} \circ \dots \circ g^{-1}}_{n \text{ copies of } g^{-1}}.$$

Then it will satisfy usual rules of indices in theorem 3-23.

WARNING Unless you know G is abelian, we can't simplify

$$(gh)^n \text{ to } g^n h^n$$

$$(gh)^n = gh \ gh \ \dots \ gh$$

Additive notation

For a known abelian group we can use the $+$ symbol for the operation.

In this we talk about/use "multiple notation"

For $n \in \mathbb{Z}$, $n \geq 0$

$$ng := g + g + \dots + g$$

Inverse elements are written as negatives. $-g$ etc.

Continue at 5:05.

Subgroups

Compare with/consider the concept of vector subspaces of a vector space.

Def If G is a group. A subset H of G ($H \subseteq G$) forms a subgroup of G if H is a group under the same operation as in G .

For any group G we can always point to two particular subgroups

The trivial subgroup $\{e\} \subset G$

The whole group G itself. $G \subseteq G$.

So of real interest will be any non-trivial proper subgroups.
ie. subgroups H

$$\{e\} \neq H \subset G \text{ but } H \neq G.$$

If indeed there are any.

Eg 3.24.

$$(\mathbb{R}^*, \cdot)$$

has the subgroup \mathbb{Q}^* , non-zero rationals



note $\mathbb{R}^* \setminus \mathbb{Q}^*$ is not a group.

- $1 \notin \mathbb{R}^+ \setminus \mathbb{Q}^+$
 - also not closed
- $$\sqrt{2} \sqrt{2} = 2 \notin \mathbb{R}^+ \setminus \mathbb{Q}^+.$$

Ex 3.25

$$H = \{1, -1, i, -i\} \subset \mathbb{C}^*.$$

forms a subgroup, here's its

Cayley

	1	-1	i	-i
1	1	-1	i	-i
-1	-1	1	-i	i
i	i	-i	1	-1
-i	-i	i	-1	1

Eg 3.26

$$SL_n(\mathbb{R}) = \{A \in GL_n(\mathbb{R}) : \det(A) = 1\}$$

forms a subgroup of $GL_n(\mathbb{R})$

Proof needs some facts from linear algebra.

Closure Given $A, B \in SL_n(\mathbb{R})$

Q $AB \in SL_n(\mathbb{R})$?

$$\begin{aligned}\det(AB) &= \det(A) \det(B) \\ &= 1 \cdot 1 \\ &= 1\end{aligned}$$

$$\Rightarrow AB \in \mathrm{SL}_n(\mathbb{R})$$

$$I \in \mathrm{SL}_n(\mathbb{R})$$

$$\text{Q is } A^{-1} \in \mathrm{SL}_n(\mathbb{R})$$

$$\begin{aligned}\det(A^{-1}) &= \frac{1}{\det(A)} \\ &= \frac{1}{1} \\ &= 1\end{aligned}$$

$$\Rightarrow A^{-1} \in \mathrm{SL}_n(\mathbb{R}).$$



Associativity on H automatically follows from the known associativity on G .

$$= (ac + 2bd) + (ad + bc)\sqrt{2}$$

$$\Rightarrow xy = \frac{\downarrow}{\in \mathbb{Q}} + \frac{\downarrow}{\in \mathbb{Q}} \sqrt{2}$$

$$\Rightarrow xy \in G$$

Both new coefficients ~~non~~ zero?

No because $xy \neq 0$. since
 $x \neq 0, y \neq 0$

3. Existence of ~~identities~~ inverses.

$$\text{Given } x = a + b\sqrt{2} \in G$$

$$\text{Is } x^{-1} \text{ in } G \text{?}$$

$$\begin{aligned} x^{-1} &= (a + b\sqrt{2})^{-1} \\ &= \frac{1}{a + b\sqrt{2}} \end{aligned}$$

, known inverse
in \mathbb{R}^*

$$\begin{aligned} \downarrow ? &= \frac{1}{a + b\sqrt{2}} \cdot \frac{a - b\sqrt{2}}{a - b\sqrt{2}}, \text{ using the conjugate of } a + b\sqrt{2} \\ &= \frac{a - b\sqrt{2}}{a^2 - 2b^2} \\ &= \frac{a}{a^2 - 2b^2} + \frac{-b}{a^2 - 2b^2} \sqrt{2} \end{aligned}$$

$$\in G \quad \checkmark.$$

So by Prop 3.30 G is a
subgroup of \mathbb{R}^* .